\documentclass[11hpt]{article}
\usepackage{amsmath}
\usepackage{mathtools}
\usepackage[all]{xy}
\usepackage{syntax}

\begin{document}

\begin{grammar}

<\lambda t> ::= \lit*{() ->} <t>
  \alt \lit*{->} <t>

<v> ::= \lit*{true}
  \alt \lit*{false}

<t> ::= <v>
  \alt <\lambda t>\lit*{()}
  \alt <\lambda t> <t>

\end{grammar}

\begin{equation}
\langle\lambda t\rangle \lit*{()} \to \langle t \rangle
\end{equation}

\begin{equation}
\langle\lambda t_{1}\rangle \ \langle t_{2} \rangle \to \langle t_{1} \rangle
\end{equation}

\begin{equation}
\frac{t : T_{1}}{\langle \lambda t \rangle: \top \to T_{1}}
\end{equation}

\begin{equation}
\dfrac{\langle\lambda t\rangle : \top \to T_{1}}{\langle\lambda t\rangle \lit*{()}: T_{1}}
\end{equation}

\begin{equation}
\frac{\langle \lambda t \rangle : \top \to T_{1} \ \ \ \langle t_{2} \rangle : T_{2} }{\langle\lambda t_{1}\rangle \ \langle t_{2} \rangle : T_{1}}
\end{equation}

\end{document}
