\documentclass[11hpt]{article}
\usepackage{amsmath}
\usepackage{mathtools}
\usepackage[all]{xy}
\usepackage{syntax}
\usepackage{trfrac}

\renewcommand{\syntleft}{\normalfont\itshape}
\renewcommand{\syntright}{}

\begin{document}

\section{Grammars}

\begin{grammar}
<e> ::= <x> | <\lambda x>.<e> | <e> <e>
\end{grammar}

\begin{grammar}
<e> ::= <x> | \lit*{(}<x>\lit*{) ->} <e> | <e> <e>
\end{grammar}

\begin{grammar}
<e> ::= <x> | <\lambda x>:<\tau>.<e> | <e> <e> | <c>
\end{grammar}

\begin{grammar}
<e> ::= <x> | \lit*{(}<x>\lit*{) -> ifft(}<x>\lit*{,}<\tau>\lit*{);} <e> | <e> <e> | <c>
\end{grammar}

\section{Lambda Calculus}

\begin{align*}
\lambda x.y \\
\lambda y.\lambda x.y \\
\lit*{(x) -> y} \\
\lit*{(y) -> (x) -> y}
\end{align*}

\begin{align*}
(\lambda y.\lambda x.y) \ \lambda z.z \quad &\rightarrow \quad \lambda x.(\lambda z.z) \\
\lit*{((y) -> (x) -> y) (z) -> z} \quad &\rightarrow \quad \lit*{(x) -> ((z) -> z)}
\end{align*}

\end{document}